progress on harmony lemma

theories/Linearity.v
@@ -1,49 +1,837 @@
-From Dep Require Import Global_Syntax.
-From mathcomp Require Import all_ssreflect.
+From mathcomp Require Import all_ssreflect zify.
 From Equations Require Import Equations.
 From mathcomp Require Import fintype.
-From deriving Require Import deriving.
 
 Set Implicit Arguments.
 Unset Strict Implicit.
 Unset Printing Implicit Defensive.
+From deriving Require Import deriving.
+Require Import Dep.Global_Syntax.
 
-Section Linearity.
-Variable (U : countType). 
-Variable (g : gType U).
-Hypotheses (Hbound : bound g) (Hcont : contractive g).
 
-Definition action_from (a : action) := let : Action p0 _ _ := a in p0.
-Definition action_to (a : action) := let : Action _ p1 _ := a in p1.
-Definition action_ch (a : action) := let : Action _ _ c := a in c.
-Definition same_ch (a0 a1 : action) := action_ch a0 == action_ch a1.
+Unset Elimination Schemes. Check seq.
+CoInductive sgType  : Type :=
+  | SGEnd : sgType  
+  | SGMsg : action -> value -> sgType -> sgType  
+  | SGBranch : action -> seq sgType -> sgType  .
+Set Elimination Schemes.
 
-Definition opt_rel (g0 g1 : gType U) (P : rel action) :=
-if act_of_g g0 is Some a0
-  then if act_of_g g1 is Some a1
+
+Inductive Forall2 (A B : Type) (R : A -> B -> Type) : seq A -> seq B -> Prop :=
+    Forall2_nil : Forall2 R nil nil | Forall2_cons : forall (x : A) (y : B) (l : seq A) (l' : seq B), R x y -> Forall2 R l l' -> Forall2 R (x :: l) (y :: l').
+Hint Constructors Forall2. Search List.Forall.
+
+Inductive Forall3 (A B C : Type) (R : A -> B -> C -> Type) : seq A -> seq B -> seq C -> Prop :=
+    Forall3_nil : Forall3 R nil nil nil | Forall3_cons : forall (x : A) (y : B) (z : C) (l : seq A) (l' : seq B) (l'' : seq C), R x y z -> Forall3 R l l' l'' -> Forall3 R (x :: l) (y :: l') (z ::l'').
+Hint Constructors Forall3.
+
+Inductive Unravel (r : gType -> sgType -> Prop) : gType -> sgType -> Prop :=
+ | UEnd : Unravel r GEnd SGEnd
+ | UMsg a u g0 sg0 : Unravel r g0 sg0 -> Unravel r (GMsg a u g0) (SGMsg a u sg0)
+ | UBranch gs sgs a : Forall2 (Unravel r) gs sgs ->  Unravel r (GBranch a gs) (SGBranch a sgs)
+ | URec g sg : r g[GRec g] sg  -> Unravel r (GRec g) sg.
+Hint Constructors Unravel.
+
+
+Require Import Paco.paco.
+Check paco2.
+
+Definition GUnroll g sg : Prop := paco2 Unravel bot2 g sg.
+
+Example test : GUnroll (GRec (GVar 0)) SGEnd.
+unfold GUnroll. pcofix CIH. pfold. constructor. right. simpl. done.
+Qed.
+Check Unravel_ind.
+Lemma Unravel_ind2
+     : forall r P : gType -> sgType -> Prop,
+       P GEnd SGEnd ->
+       (forall (a : action) (u : value) (g0 : gType) (sg0 : sgType),
+        Unravel r g0 sg0 -> P g0 sg0 -> P (GMsg a u g0) (SGMsg a u sg0)) ->
+       (forall (gs : seq gType) (sgs : seq sgType) (a : action),
+        Forall2 (Unravel r) gs sgs -> Forall2 P gs sgs -> P (GBranch a gs) (SGBranch a sgs)) ->
+       (forall (g : gType) (sg : sgType), r (g)[GRec g] sg -> P (GRec g) sg) ->
+       forall (g : gType) (s : sgType), Unravel r g s -> P g s.
+Proof.
+intros. move : g s H3. fix IH 3. move => g s [].
+- apply H.
+- intros. apply H0. apply u0.  apply IH. apply u0. 
+- intros. apply H1. apply f.
+- induction f.  done. constructor. apply IH. apply H3. apply IHf. 
+- intros. apply H2. apply r0.
+Qed.
+
+Lemma GUnroll_mono : monotone2 Unravel.
+Proof.
+elim;intros.
+-  inversion IN. 
+- inversion IN. auto. 
+- inversion IN. subst. auto.  
+- inversion IN. eauto.  
+- inversion IN. subst. constructor. move : l sgs IN H3 H. elim. 
+ + intros. inversion H3. auto.
+ + intros. inversion H3. subst. constructor. eapply H0.  by  rewrite inE eqxx. eauto. eauto. eauto.
+   apply H. constructor. auto. auto.  intros.  eapply H0. by rewrite inE H1 orbC. eauto. eauto. 
+Qed.
+Hint Resolve GUnroll_mono : paco.
+
+Definition label := (action * (value + nat))%type.
+(*Inductive label := 
+ | LU : action -> value -> label
+ | LN : action -> nat -> label. 
+
+Notation nth_error := List.nth_error.  *)
+
+
+(*Inductive DAfter : sgType -> label ->  sgType -> Prop :=
+ | DMsg a u sg : DAfter (SGMsg a u sg) (LU a u) sg
+ | DBranch a g gs i : nth_error gs i = Some g -> DAfter (SGBranch a gs) (LN a i) g.
+
+Inductive After : sgType -> seq label -> sgType -> Prop := 
+ | After_0 sg : After sg nil sg
+ | After_step a a_s sg0 sg1 sg2 : DAfter sg0 a sg1 -> After sg1 a_s sg2 -> After sg0 (a::a_s) sg2.
+
+Definition act_of_sg sg :=
+match sg with 
+| SGEnd => None
+| SGMsg a _ _ => Some a
+| SGBranch a gs => Some a
+end.
+
+Definition opt_rel_sg (P : rel action)  (g0 g1 : sgType) :=
+if act_of_sg g0 is Some a0
+  then if act_of_sg g1 is Some a1
     then P a0 a1
   else false 
-else false.
+else false.*)
+
+Definition same_ch (a0 a1 : action) := action_ch a0 == action_ch a1.
+
+Definition II (a0 a1 : action) := (ptcp_to a0 == ptcp_to a1).
+Definition IO (a0 a1 : action) := (ptcp_to a0 == ptcp_from a1).
+Definition OO (a0 a1 : action) := (ptcp_from a0 == ptcp_from a1) && same_ch a0 a1.
+Definition IO_OO a0 a1 := IO a0 a1 || OO a0 a1.
+
+Inductive InDep : seq action -> Prop :=
+ | ID_End a0 a1 : II a0 a1 -> InDep ([::a0; a1])
+ | ID_cons a0 a1 aa: IO a0 a1 -> InDep (a1::aa) -> InDep (a0::a1::aa).
+Hint Constructors InDep.
+
+(*Fixpoint indep ss := 
+match ss with 
+| a::s' => match s' with 
+         | a'::nil => II a a'
+         | a'::s'' => (IO a a') && (indep s')
+         | _ => false
+         end
+| _ => false
+end.*)
+
+Definition indep ss := 
+match ss with 
+| a::a'::ss' => let: one_less := belast a' ss' in path IO a one_less && II (last a one_less) (last a' ss')
+| _ => false 
+end.
+
+Lemma InDep_iff : forall ss, InDep ss <-> indep ss.
+Proof.
+case. split;intros;inversion H.
+move => a l. case : l. split;intros;inversion H.
+move => a0 l. 
+elim : l a0 a. rewrite /=. move => a0 a. split;intros; inversion H;subst. done. inversion H4. auto.
+move => a0 l H a1. rewrite /=. split;intros.
+- inversion H0;subst. rewrite H3 /=. simpl in H. by  apply/H.
+- move : H0 => /andP => [] [] /andP => [] []. intros. constructor. done. apply/H. by rewrite /= b b0.
+Qed.
+
+Inductive OutDep : seq action -> Prop :=
+ | OD_end a0 a1 : IO_OO a0 a1 -> OutDep ([::a0; a1])
+ | OD_cons a0 a1 aa: IO_OO a0 a1  -> OutDep (a1::aa) -> OutDep (a0::a1::aa).
+Hint Constructors OutDep.
+
+Fixpoint dep (R : action -> action -> bool) ss := 
+match ss with 
+| nil => false 
+| a::s' => match s' with 
+          | a'::nil => R a a' 
+          | a'::ss' => (R a a') && dep R s'
+          | _ => false
+        end
+        
+end.
+
+Definition outdep ss :=
+match ss with 
+| a::a'::ss => path IO_OO a (a'::ss)
+| _ => false 
+end. 
+
+Lemma OutDep_iff : forall ss, OutDep ss <-> outdep ss.
+Proof.
+rewrite /outdep.
+case; first (split;intros; inversion H).
+move => a []; first (split;intros;inversion H).
+move => a0 l. move : l a a0. elim.
+- move => a a0. split; rewrite /=;intros. rewrite andbC /=. inversion H; done.
+  constructor. by move : H => /andP => [] [].
+- move => a l IH a0 a1. split;intros. 
+ * inversion H. subst. rewrite /=. simpl in IH. rewrite H2 /=. inversion H4;subst. by rewrite H1. 
+   by apply/IH. 
+ * simpl in IH,H. move : H=> /andP=> [] []H0 H1. constructor;first done. by apply/IH.  
+Qed.
+(*Notation outdep := (dep (fun a0 a1 => IO a0 a1 || OO a0 a1)).
+
+Lemma OutDep_iff : forall ss, OutDep ss <-> outdep ss.
+Proof.
+elim.
+- rewrite /=. split;intros;inversion H.
+- move => a l H. split;intros. 
+ * rewrite /=. case : l H0 H. 
+  ** intros. inversion H0. 
+  ** intros. case : l H H0. 
+   *** intros. inversion H0. apply/orP. done. 
+   *** apply/orP.  done. 
+ * intros. apply/andP. rewrite -H. inversion H0. split. apply/orP. done. done. 
+ 
+ simpl in H0. case : l H H0. 
+ *  done. 
+ * move => a0 l H [].
+  ** case : l H. 
+   *** intros. constructor. by apply/orP.
+   *** move => a1 l H /andP. move => [] H2 H3.  constructor.  apply/orP. done. apply/H. done. 
+Qed.*)
+
+Ltac contra_list := match goal with 
+                      | H : (nil = _ ++ _) |-  _ => apply List.app_cons_not_nil in H
+                      end;contradiction.
+
+(*Definition OutDep2 (s : seq action) := exists a a' s', s = a::a'::s' /\ path ((fun a0 a1 => (IO a0 a1) || (OO a0 a1))) a (a'::s').*)
+(*
+Lemma OutDep_iff : forall aa, OutDep aa <-> OutDep2 aa.
+Proof.
+rewrite /OutDep2. elim.
+- split. intros. inversion H. move => [] a [] a' [] x []. intros.  inversion a0. 
+- intros. split.
+ * intros. inversion H0. subst. exists a,a1,nil. rewrite /= andbC /=. split. done. apply/orP. done. 
+ * subst. apply H in H4.  move : H4 => [] a0 [] a' [] s' [] []. intros.  subst. exists a0,a',s'. split. subst. rewrite /=. split. done. apply/andP. split. apply/orP. done. 
+   applymove => [] a2 [] a' [] s'. [::a1]. split;auto. rewrite /=. rewrite andbC /=. apply/orP. done. done.
+ * subst. apply H in H4. case : H4. move => [] a0 [] s' [] HH0 HH1 Hlt.  split. exists a. exists (a0::s'). rewrite HH0.  split;auto. 
+   rewrite /=. case : HH0.  intros. subst. apply/andP. split. apply/orP. done. done. done. 
+
+ * move => [] [] a0 [] s' [] HH0 HH1 Hlt. inversion HH0. subst. case : s' HH0 H HH1 Hlt. 
+  ** intros. done. 
+  ** simpl. intros. move : (andP HH1)=> []. move/orP. intros. constructor. done. apply/H. split. exists a. exists l. auto. exists a. a0 s'. subst. intros. case : a0. move : (H H4). split. exists a , (a1::aa). split;auto. rewrite /=.*)
+
+(*Definition label_indDef := [indDef for label_rect].
+Canonical label_indType := IndType label label_indDef.
+Definition label_eqMixin := [derive eqMixin for label].
+Canonical label_eqType := EqType label label_eqMixin.*)
+
+Definition in_action p a := let: Action p0 p1 k :=a in  (p==p0) || (p==p1).
+
+Coercion to_action (l : label) : action := l.1.
+
+(*Definition act_of_label l := 
+match l with 
+| LU a _ => a
+| LN a _ => a
+end.*)
+
+Definition pred_of_label (l : label) : {pred ptcp} := fun p => in_action p l.
+
+Canonical label_predType := PredType pred_of_label. 
 
 
 
-Definition II_aux (a0 a1 : action) := (action_to a0 == action_to a1).
-Definition II_spec (g0 g1 : gType U) := (grel g_next g0 g1) && opt_rel g0 g1 II_aux. 
+Inductive Tr : seq action -> sgType -> Prop :=
+| TR_nil G : Tr nil G 
+| TRMsg a u aa g0 : Tr aa g0 -> Tr (a::aa) (SGMsg a u g0)
+| TRBranch a gs n aa : Tr aa (nth SGEnd gs n) ->  Tr (a::aa) (SGBranch a gs).
+Hint Constructors Tr.
+(*Fixpoint tr (ls : seq action) (sg : sgType)  {struct ls}  :=
+match sg,ls with 
+| _,nil => true
+| SGMsg a u sg', a'::nil => (a == a')
+| SGBranch a sgs, a'::nil => (a == a')
+| SGMsg a u sg', a'::ls' => (a == a') && (tr ls' sg')
+| SGBranch a sgs, a'::ls' => (a == a') && has (fun g => tr ls' g) sgs
+| _,_ => false
+end.*)
 
-Definition IO_aux (a0 a1 : action) := (action_to a0 == action_from a1).
-Definition IO_spec (g0 g1 : gType U) := (grel g_next g0 g1) && opt_rel g0 g1 IO_aux. 
 
-Definition OO_aux (a0 a1 : action) := (action_from a0 == action_from a1) && (action_ch a0 == action_ch a1).
-Definition OO_spec (g0 g1 : gType U) := (grel g_next g0 g1) && opt_rel g0 g1 OO_aux. 
+(*Definition trace_clash aa' := exists a0 aa a', aa' = a0::(rcons aa a') /\ same_ch a0 a'.*)
 
-Definition in_dep_spec (g0 g1 : gType U) := (exists (g' : gType U), (exists2 p, path IO_spec g0 p & g' = last g0 p) /\ II_spec g' g1) 
-                                      \/ II_spec g0 g1.
+(*Definition Linear (sg : sgType) := forall aa_p a0 aa a1, Tr (aa_p ++ (a0::aa++[::a1])) sg -> same_ch a0 a1 -> 
+exists mi mo, size mi = size mo /\ size mi = size aa /\ InDep (a0::((mask mi aa)++[::a1])) /\ 
+                                                OutDep (a0::((mask mo aa))++[::a1]).*)
+Definition exists_depP  (Pm : seq bool -> Prop) (P : seq action -> Prop) a0 aa a1 := exists m, size m = size aa /\ P (a0::((mask m aa))++[::a1]) /\ Pm m.
+Notation exists_dep := (exists_depP (fun _ => True)).
 
-Definition OO_IO_spec (g g' : gType U) := OO_spec g g' || IO_spec g g'.
-Definition out_dep_spec(g0 g1 : gType U) := exists2 p, path OO_IO_spec g0 p & g1 = last g0 p.
 
-Definition linear_spec := 
-forall (g0 g1 : gType U), (exists2 p, path (grel g_next) g p & g0 = last g p) ->
-                     (exists2 p, path (grel g_next) g0 p & g1 = last g0 p) ->
-                     opt_rel g0 g1 same_ch -> in_dep_spec g0 g1 /\ out_dep_spec g0 g1.
-End Linearity. 
+Definition Linear (sg : sgType) := forall aa_p a0 aa a1, 
+Tr (aa_p ++ (a0::aa++[::a1])) sg -> 
+same_ch a0 a1 -> 
+exists_dep InDep a0 aa a1 /\ exists_dep OutDep a0 aa a1.
+Print sum.
+Definition value_nat := (@sum value nat).
+Identity Coercion value_nat_coercion : value_nat >-> sum.
+
+(*FunClass coercion*)
+(*Parameter (c : ch) (p : ptcp). Check Action.
+Inductive my_prod (A B : Set) := my_pair : A -> B -> my_prod A B.
+Coercion nat_value_nat (n : nat) :  @sum value nat := inr n.
+Coercion value_value_nat (v : value) :  @sum value nat := inl v.
+Parameter (a : action).
+Check (0 : value_nat).
+Definition my_prod2 := @prod action value_nat. Print prod.
+
+Check (my_pair a 0 : my_prod action value_nat).  : (nat * bool) % type).
+
+
+
+Check ((0, true) : value_nat* true).
+Definition action_vn := @prod action value_nat.
+Identity Coercion prod_coercion : action_vn >-> prod.
+
+Coercion nat_test : (a : action) (n : nat) *)
+Unset Elimination Schemes. 
+Inductive step : sgType -> label  -> sgType -> Prop :=
+ | GR1 (a : action) u g : step (SGMsg a u g) (a, inl u) g
+ | GR2 a n d gs : n < size gs -> step (SGBranch a gs) (a, inr n) (nth d gs n)
+ | GR3 a u l g1 g2 : step g1 l g2 -> ptcp_to a \notin l -> step (SGMsg a u g1) l (SGMsg a u g2)
+ | GR4 a l gs gs' : Forall2 (fun g g' => step g l g') gs gs' -> (ptcp_to a) \notin l  ->  step (SGBranch a gs) l (SGBranch a gs').
+Set Elimination Schemes. 
+Hint Constructors step. 
+
+Lemma step_ind
+     :  forall P : sgType -> label -> sgType -> Prop,
+       (forall (a : action) (u : value) (g : sgType), P (SGMsg a u g) (a, inl u) g) ->
+       (forall (a : action) (n : nat) (d : sgType) (gs : seq sgType),
+        n < size gs -> P (SGBranch a gs) (a, inr n) (nth d gs n)) ->
+       (forall (a : action) (u : value) (l : label) (g1 g2 : sgType),
+        step g1 l g2 ->
+        P g1 l g2 -> ptcp_to a \notin l -> P (SGMsg a u g1) l (SGMsg a u g2)) ->
+       (forall (a : action) (l : label) (gs gs' : seq sgType),
+        Forall2 (fun g : sgType => step g l) gs gs' ->  Forall2 (fun g0 g2 : sgType => P g0 l g2) gs gs' -> 
+
+        ptcp_to a \notin l -> P (SGBranch a gs) l (SGBranch a gs')) ->
+       forall (s : sgType) (l : label) (s0 : sgType), step s l s0 -> P s l s0.
+Proof.
+move => P H0 H1 H2 H3. fix IH 4.
+move => ss l s1 [].
+intros. apply H0;auto. 
+intros. apply H1;auto.
+intros. apply H2;auto.
+intros. apply H3;auto. elim : f;auto.  
+Qed.
+
+
+Unset Elimination Schemes. 
+Inductive stepG : sgType -> sgType -> label  -> sgType -> Prop :=
+| GGR1 a u g0 : stepG (SGMsg a u g0) (SGMsg a u SGEnd) (a, inl u) g0
+| GGR2 a d gs n : n < size gs -> stepG (SGBranch a gs) (SGBranch a nil) (a, inr n) (nth d gs n)
+| GGR3 a u  g G l g' : stepG g G l g'  -> (ptcp_to a) \notin l ->
+                     stepG (SGMsg a u g) (SGMsg a u G) l (SGMsg a u g')
+| GGR4 a gs GS gs' l : Forall3 (fun g G g' => stepG g G l g') gs  GS gs' -> (ptcp_to a) \notin l -> stepG (SGBranch a gs) (SGBranch a GS) l (SGBranch a gs').
+Hint Constructors stepG.
+Set Elimination Schemes. 
+Lemma stepG_ind
+     : forall P : sgType -> sgType -> label -> sgType -> Prop,
+       (forall (a : action) (u : value) (g0 : sgType),
+        P (SGMsg a u g0) (SGMsg a u SGEnd) (a, inl u) g0) ->
+       (forall (a : action) (d : sgType) (gs : seq sgType) (n : nat),
+        n < size gs -> P (SGBranch a gs) (SGBranch a nil) (a, inr n) (nth d gs n)) ->
+       (forall (a : action) (u : value) (g G : sgType) (l : label) (g' : sgType),
+        stepG g G l g' ->
+        P g G l g' ->
+        ptcp_to a \notin l -> P (SGMsg a u g) (SGMsg a u G) l (SGMsg a u g')) ->
+       (forall (a : action) (gs GS gs' : seq sgType) (l : label),
+        Forall3 (fun g G : sgType => stepG g G l) gs GS gs' ->
+        Forall3 (fun g G g' : sgType => P g G l g' ) gs GS gs' ->
+        ptcp_to a \notin l -> P (SGBranch a gs) (SGBranch a GS) l (SGBranch a gs')) ->
+       forall (s s0 : sgType) (l : label) (s1 : sgType), stepG s s0 l s1 -> P s s0 l s1.
+Proof.
+move => P H0 H1 H2 H3. fix IH 5.
+move => ss s0 l s1 [].
+intros. apply H0;auto. 
+intros. apply H1;auto.
+intros. apply H2;auto.
+intros. apply H3;auto. elim : f. done. intros. constructor. apply IH. done. done.
+Qed.
+
+
+(*Should be split into pred and size lemmas*)
+Lemma Forall3_forall_n : forall A B C (P : A -> B -> C -> Prop) (l0 : seq A) (l1 : seq B) (l2 : seq C) da db dc, Forall3 P l0 l1 l2 -> (forall n, n < size l0 -> P (nth da l0 n) (nth db l1 n) (nth dc l2 n)) /\ size l0 = size l1 /\ size l1 = size l2.  
+Proof.
+intros. elim : H. rewrite /=. split;auto. intros.  done.
+rewrite /=. intros. move : H1 => [] H2 [] H3 H4. split;auto. case. rewrite /=. done. move => n. rewrite /=.
+intros. have : n < size l. done. intros. apply H2. done. 
+Qed.
+
+Lemma Forall3_forall_n_def : forall A B C (P : A -> B -> C -> Prop) (l0 : seq A) (l1 : seq B) (l2 : seq C) da db dc, P da db dc -> Forall3 P l0 l1 l2 -> (forall n, n <= size l0 -> P (nth da l0 n) (nth db l1 n) (nth dc l2 n)) /\ size l0 = size l1 /\ size l1 = size l2.  
+Proof.
+intros. elim : H0. rewrite /=. split;auto. intros.  rewrite !nth_nil. done.
+rewrite /=. intros. move : H2 => [] H4 [] H5 H6. split;auto. case. rewrite /=. done. move => n. rewrite /=.
+intros. have : n <= size l. done. auto.  
+Qed.
+
+
+
+Lemma step_G : forall g l g',  step g l g' -> exists G, stepG g G l g'.
+Proof. 
+fix IH 4. intros. case : H; try solve [intros;econstructor;eauto].
+- intros. case  : (IH _ _ _ s). intros. exists (SGMsg a u x). eauto. 
+- intros. 
+ have : exists GS, Forall3 (fun g G g' => stepG g G l0 g') gs GS gs'. 
+ * elim : f.
+  **  exists nil. done. 
+  **  intros. case : (IH _ _ _ H).  intros. case : H1. intros. exists (x0::x1). eauto. 
+ *  case. intros. exists (SGBranch a x);eauto. 
+Qed.
+
+Lemma G_step : forall g G l g', stepG g G l g' -> step g l g'.
+Proof.
+fix IH 5. 
+intros. case : H; try solve [intros;constructor;auto].
+intros. constructor;eauto. Guarded. 
+intros. constructor. elim : f. done. intros. constructor. eauto. 
+done. done. 
+Qed.
+
+Lemma linear_sgmsg : forall a u g0, Linear (SGMsg a u g0) -> Linear g0.
+Proof. 
+move => a u g0. rewrite /Linear /=.  intros. move : (H (a::aa_p) a0 aa a1). rewrite cat_cons /=. 
+  destruct ( aa_p ++ a0 :: rcons aa a1) eqn:Heqn. case : aa_p H0 Heqn.  done. done.
+  intros. have : Tr ((a::aa_p ++ (a0::aa) ++ [::a1])) (SGMsg a u g0). auto.  move/H2 => H3.  move : (H3 H1). 
+  move => [] mi [] mo. intros. auto. 
+Qed.
+
+Lemma nth_def : forall A (l : seq A) n d0 d1 , n < size l -> nth d0 l n = nth d1 l n.
+Proof.
+move => A. elim.
+- case;done. 
+intros. case : n H0. done. rewrite /=. intros. apply H. done. 
+Qed.
+
+Lemma linear_branch : forall a gs, Linear (SGBranch a gs) -> forall n d, n < size gs -> Linear (nth d gs n).
+Proof.
+intros. rewrite /Linear. intros. unfold Linear in H. have : Tr (a::aa_p ++ a0::aa ++ ([::a1])) (SGBranch a gs). eauto. 
+intros. apply TRBranch with (n:=n). erewrite nth_def. eauto. done. intros. apply : H. move : x. rewrite -cat_cons. intros. apply : x. done. 
+Qed.
+
+
+
+
+Lemma Tr_reduce : forall  G g l g', stepG g G l g' -> forall s, Tr s G -> Tr s g.
+Proof.
+intros. move :  H s H0.  elim. 
+- intros. inversion H0. done. subst. inversion H2. subst. eauto.   
+- intros.  inversion H0.  done. subst. move : H3. rewrite nth_nil.  intros. inversion H3. subst. apply TRBranch with (n:=0). 
+  done. 
+- intros. inversion H2.  done. subst. constructor. eauto.  
+- intros. inversion H2. subst. done. subst.
+  move : (@Forall3_forall_n _ _ _ _ gs GS gs' SGEnd SGEnd SGEnd H0) => [] H8 [] H9 H10.  
+
+(*move : (@Forall3_forall_n _ _ _ (fun g0 g1 => fun _ => forall s, Tr s g1 -> Tr s g0) gs GS gs' d d d H0)=> [] H8 [] H9 H10.  *)
+  case Heq : (n < size gs). 
+ * move : (H8 n Heq). intros. apply TRBranch with (n:=n). apply H3. done. 
+   have : size GS <= n. lia. intros. move : H5.  rewrite nth_default //=. intros. inversion H5. subst.
+   apply TRBranch with (n:=n).  rewrite nth_default //=. rewrite H9. done. 
+Qed.
+Print stepG.
+
+Lemma label_linear : forall g G l g',  stepG g G l g' -> Linear g -> Linear G.
+Proof.
+move => g G l g'. elim.
+- move => a u g0 _.  rewrite /Linear. case. rewrite /=. intros. inversion H. subst. inversion H2. case : aa H H2 H3;done. 
+  move => a0 l0 a1 aa a2. rewrite cat_cons. intros. inversion H. subst. inversion H2. apply List.app_cons_not_nil in H3.   done.
+- move => a _ gs n Hlt HL. rewrite /Linear. intros. inversion H. apply List.app_cons_not_nil in H2. done. 
+  subst. move : H3. rewrite nth_nil. intros. inversion H3. subst. exfalso. 
+  clear H H0 H3.
+  case : aa_p H1. rewrite /=. case. move => _ H3. apply List.app_cons_not_nil in H3. done.
+  move => a2 l0.  rewrite cat_cons. case. move => _ H3. apply List.app_cons_not_nil in H3. done.
+- move => a u g0 G0 l0 g'0. intros.  move : (linear_sgmsg H2). move/H0=> H3. 
+  have : stepG (SGMsg a u g0) (SGMsg a u G0) l0 (SGMsg a u g'0). eauto. 
+  move/Tr_reduce=> H4. move : H2. rewrite /Linear. 
+  intros. apply : H2; eauto. 
+- intros. have : stepG (SGBranch a gs) (SGBranch a GS) l0 (SGBranch a gs'). eauto. move/Tr_reduce=>H3.
+  move : H2.  rewrite /Linear. intros. eauto.  
+Qed.
+
+
+
+Lemma Tr_or : forall s g, Tr s g \/ ~ (Tr s g).
+Proof.
+elim. intros. auto. 
+intros. case : g. 
+- right. move => H2. inversion H2. 
+- intros. case : (H s).  case (eqVneq a a0). move =>->. auto. 
+  right. move => H2. inversion H2. apply (negP i). by apply/eqP. 
+- intros. right. move => H2. inversion H2. done. 
+  intros. case : (eqVneq a a0). 
+ * move => ->. elim : l0. case : l H.  intros. left. auto. apply TRBranch with (n:=0). rewrite nth_nil. done. 
+   intros. right. move => H2. inversion H2.  rewrite nth_nil in H1. inversion H1. 
+   intros. case : H0.  
+  ** intros. left. inversion a2. subst. apply TRBranch with (n:=n.+1). rewrite /=. done. 
+  ** intros. case : (H a1). intros. left. apply TRBranch with (n:=0).  done. 
+     intros. right. move => H2. apply b. inversion H2. subst.  case : n H1. rewrite /=. done.
+     intros. apply TRBranch with (n:=n). done. 
+ * move/eqP=>H2. right. move => H3. apply H2. inversion H3. done. 
+Qed.
+
+
+
+Definition app_Forall3 {P : sgType -> sgType -> sgType -> Prop}{gs GS gs' : seq sgType} (H : Forall3 P gs GS gs') := @Forall3_forall_n _ _ _ _ gs GS gs' SGEnd SGEnd SGEnd H.
+
+
+Definition app_Forall3_def {P : sgType -> sgType -> sgType -> Prop}{gs GS gs' : seq sgType}  (H : Forall3 P gs GS gs') (H0 : P SGEnd SGEnd SGEnd) := @Forall3_forall_n_def _ _ _ _ gs GS gs' SGEnd SGEnd SGEnd H0 H.
+
+
+
+Lemma reduce_condition : forall g G l g', stepG g G l g' -> forall aa a' a, Tr (aa++([::a])) G ->  
+a' \in aa -> (ptcp_to a') \notin l.  
+Proof.
+move => g G l g'. elim.
+- intros. case : aa H H0; first done.  move => a1 l0. rewrite /=. intros. inversion H. subst. 
+  inversion H2. contra_list. 
+- intros.  case : aa H H0 H1; first done.  move => a1 l0. rewrite /=. intros. inversion H0. subst. 
+  rewrite nth_nil in H3. inversion H3. contra_list.
+- intros. case : aa H2 H3. done. move => a1 l1. rewrite cat_cons. intros. inversion H2. subst.
+  move : H3. rewrite inE. move/orP=>[ /eqP ->  |  ]. done.  eauto. 
+- intros. case : aa H2 H3. done. move => a1 l1. rewrite cat_cons. intros. 
+  move : H3. rewrite inE. move/orP=>[ /eqP ->  |  ]. inversion H2.  subst. eauto.
+  move : (app_Forall3 H0)=> []. intros. inversion H2.  subst.
+  case Heq : (n < size gs). apply : a2. eauto. eauto. done. 
+  rewrite nth_default in H4. inversion H4. contra_list. lia.
+Qed.
+Check TRBranch.
+Definition TRBranchn {gs aa} n a (H : Tr aa (nth SGEnd gs n)) := @TRBranch a gs n aa H.
+Check TRBranchn.
+Arguments TRBranchn {_} {_} n.
+Check TRBranchn.
+
+
+Lemma deletion : forall g G l g', stepG g G l g' -> forall s, Tr s g' -> ~ Tr s G -> exists s0 s1, s = s0++s1 /\ Tr (s0++(l.1)::s1) g /\ Tr (s0++([::l.1])) G.
+Proof. 
+move => g G l g'. elim.
+- intros. exists nil. exists s. rewrite /=. auto.
+- intros. exists nil. exists s. rewrite /=. split;auto. split. apply TRBranch with (n:=n). 
+  move : H0. rewrite (nth_def _ SGEnd) //=. apply TRBranch with (n:=0).  done. 
+- intros. inversion H2. 
+ * subst. exfalso. apply H3. done. 
+ * subst. have : ~Tr aa G0.  move => H7. apply H3. auto. move => H7. 
+   move : (H0 aa H6 H7)=> [] s0 [] s1 [] -> H8. exists (a::s0). exists s1. rewrite cat_cons. split;auto.  rewrite cat_cons. auto. case : H8. intros. rewrite cat_cons. auto. 
+- intros. inversion H2. subst. 
+ *  exists nil. exists nil. rewrite /=. exfalso. eauto. 
+ * subst. move :  (@Forall3_forall_n _ _ _ _ gs GS gs' SGEnd SGEnd SGEnd H0).   
+   move => [] Hall Hsize.
+   have : ~Tr aa (nth SGEnd GS n). move => HH. apply H3. eauto. move => HH.
+   case Heq : (n < size gs).
+   move : (Hall n Heq aa H6 HH)=> [] s0 [] s1 [] -> [] HH0 HH1. 
+   exists (a::s0). exists s1. rewrite /=. eauto. 
+   rewrite nth_default in H6. inversion H6.  subst. rewrite nth_default in HH. done. 
+   lia. lia. 
+Qed.
+
+
+Lemma split_list : forall A (l : seq A), l = nil \/ exists l' a, l = l'++([::a]).
+Proof.
+move => A. elim.
+auto.  move => a l [] . move =>->. right.  exists nil. exists a. done. 
+move => [] l' [] a0 ->. right. exists (a::l'). exists a0. done.
+Qed.
+
+Lemma Tr_app : forall l0 l1 G, Tr (l0++l1) G -> Tr l0 G.
+Proof.
+elim. rewrite /=. done.
+move => a l IH l1 G. rewrite cat_cons. move => H. inversion H. 
+- subst. constructor. eauto.  
+- subst. apply TRBranch with (n:=n). eauto.
+Qed.
+
+Lemma last_eq : forall A (l0 l1 : seq A) x0 x1, l0 ++ ([::x0]) = l1 ++ ([::x1]) -> l0 = l1 /\ x0 = x1.
+Proof.
+move => A. elim.
+case. rewrite /=. move => x0 x1. case. done.
+move => a l x0 x1. rewrite /=. case. move =>-> H. apply List.app_cons_not_nil in H. done. 
+rewrite /=. intros. case : l1 H0.  rewrite /=. case. move => _ /esym H1. apply List.app_cons_not_nil in H1. done. 
+intros. move : H0.  rewrite cat_cons. case. intros. move : (H _ _ _ H1). case. intros. split. subst. done. done. 
+Qed.
+
+
+  
+
+Lemma split_mask : forall A (l0 : seq A) x l1 m, size m = size (l0++x::l1) ->
+mask m (l0 ++ x :: l1) =
+  mask (take (size l0) m) l0 ++ (nseq (nth false m (size l0)) x) ++ mask (drop (size l0).+1 m) l1.
+Proof.
+move => A. elim. 
+- rewrite /=. intros. rewrite take0 /=. case : m H. done. 
+  intros. by  rewrite mask_cons /= drop0. 
+- rewrite /=. intros. case : m H0.  done. rewrite /=. intros. 
+  case : a0. rewrite cat_cons. f_equal. rewrite H //=. lia. 
+  rewrite H //=. lia.
+Qed.
+
+Lemma add_sub : forall n1 n0, n0 = n0 + n1 - n1. 
+elim.
+lia. 
+intros. lia. 
+Qed.
+
+Lemma in_mem_action_p : forall (p1 : ptcp) p2 c0 b, p1 \in ((Action p1 p2 c0, b): label).
+Proof.
+intros. rewrite /in_mem /=. by rewrite /pred_of_label /= eqxx. Qed.
+
+Lemma in_mem_action_p2 : forall (p1 : ptcp) p2 c0 b, p2 \in ((Action p1 p2 c0, b): label).
+Proof.
+intros. rewrite /in_mem /=. by rewrite /pred_of_label /= eqxx orbC. Qed.
+
+
+Hint Resolve in_mem_action_p in_mem_action_p2.
+
+Lemma contra1 : forall a (l0 : label), II a l0 -> (ptcp_to a) \notin l0 -> False.
+Proof.
+case. move => p p0 c []; rewrite /II /=;intros; apply : (negP H0).   destruct a. simpl in H. rewrite (eqP H). auto. 
+Qed.
+
+Lemma contra2 : forall a (l0 : label), IO a l0 -> (ptcp_to a) \notin l0 -> False.
+Proof.
+case. move => p p0 c []; rewrite /IO /=;intros; apply : (negP H0). destruct a. simpl in H.  rewrite (eqP H). auto. 
+Qed.
+
+Lemma split_indep : forall s a0 a1 s2, InDep (s++a0::a1::s2) -> InDep (a0::a1::s2).
+Proof.
+elim. auto. rewrite /=. intros. apply H. inversion H0. subst. case : l H3 H0 H.  rewrite /=. intros. done.
+rewrite /=. intros. case : H3. intros. apply List.app_cons_not_nil in H3. done. done.
+Qed.
+
+Lemma in_action_to : forall a, in_action (ptcp_to a) a.
+Proof.
+case. intros. by rewrite/= eqxx orbC.
+Qed. 
+
+Lemma in_action_from : forall a, in_action (ptcp_from a) a.
+Proof.
+case. intros. by rewrite/= eqxx.
+Qed. 
+
+Lemma cons23 : forall A  s0 s1 aa (a0 : A) a1,  a0 :: aa ++ [:: a1] = s0 ++ s1 -> s0 = nil /\ a0::aa++([:: a1]) = s1 \/ s1 = nil /\  a0::aa++([:: a1]) = s0 \/ exists s0' s1', s0 = a0::s0' /\ s1 = s1'++([::a1]) /\ s0' ++ s1' =  aa.
+Proof.
+move => A. elim.
+move => s1 aa a0 a1. rewrite /=. move => <-. auto. 
+rewrite /=. intros. case : H0. move => <-. case : aa. rewrite /=. case : s1. rewrite cats0. move => <-. auto. 
+move => a2 l0. right. right. exists l. case : l H H0. rewrite /=. intros. exists nil. done. 
+rewrite /=. intros. case : H0.  intros. apply List.app_cons_not_nil in H1. done. 
+move => a2 l0. rewrite cat_cons. move/H. case. 
+- case. move => -> <-. right. right. exists nil. exists (a2::l0). done. 
+case. 
+ - case. move => -> <-. auto. 
+ - case.  move => x [] x1 [] -> [] -> H1. right. right. exists (a2::x). exists x1. rewrite /= H1. done. 
+Qed.
+
+
+Lemma InDep_app : forall l0 l1, InDep (l0 ++ l1) -> 1 < size l1 -> InDep l1.
+Proof.
+elim. rewrite /=. done.
+move => a l IH l1. rewrite cat_cons. move => H. inversion H. subst.
+case : l H2 H IH.  rewrite /=. move => <-. done. 
+move => a0 l. rewrite cat_cons. case. move => <-. case : l.  case : l1. done. done. done. 
+intros. subst. rewrite H1 in H3. auto. 
+Qed.
+
+Definition IO_II a0 a1 := IO a0 a1 || II a0 a1.
+
+Lemma ind_aux : forall l a a0, path IO a (belast a0 l) -> II (last a (belast a0 l)) (last a0 l) -> IO_II a a0 && path IO_II a0 l.
+Proof.
+ elim.
+- move => a a0.  rewrite /= /IO_II. move => _ ->.  by rewrite orbC.
+- move => a l IH a0 a1. rewrite /=. move/andP=>[].  intros. rewrite /IO_II a2 /=.
+  unfold IO_II in IH. apply/IH. done. done. 
+Qed.
+
+Lemma indep0 : forall l0 l1, indep (l0 ++ l1) -> if l0 is x::l0' then path IO_II x l0' else true.
+Proof.
+move => l0 l1. rewrite /indep.
+case :l0 ;first done.
+move => a l. rewrite /=. case : l;first done.
+move => a0 l. rewrite /=. move/andP=> [] H H1. elim : l a a0 H H1.
+- move => a a0. rewrite /=.  case : l1. simpl. rewrite /IO_II. move => _ -> . by rewrite orbC.  
+  move => a1 l. rewrite/= /IO_II. by move/andP=> [] ->.
+- move => a l IH a0 a1. rewrite /= /IO_II. move/andP=> [] ->. intros. rewrite /=. 
+  unfold IO_II in IH. apply/IH. done. done.
+Qed.
+
+
+Lemma indep1 : forall l0 l1, indep (l0 ++ l1) -> if l1 is x::l1' then path IO_II x l1' else true.
+Proof.
+case. simpl. case. done. rewrite /=. move => a []. done.
+move => a0 l. rewrite /=. intros. move : H. move/andP=>[]. intros. apply/ind_aux. done. done. 
+- move => a l l1. rewrite /=. case : l. rewrite /=. case : l1. done.
+  intros. move : H=> /andP=> [] []. intros. move : (ind_aux a1 b). by move/andP=>[].
+- move => a0 l. rewrite /=. move/andP=> []. intros. case : l1 a1 b. done. 
+intros. move : (ind_aux a2 b). move/andP=> []. rewrite cat_path. move => _ /andP => [] []. 
+  rewrite /=. move => _ /andP => [] []. done. 
+Qed.
+
+
+Inductive IO_seq : seq action -> Prop :=
+ | IO_seq0 a b : IO a b ->  IO_seq ([::a; b])
+ | IO_seq1 a b l : IO a b -> IO_seq (b::l) -> IO_seq (a::b::l).
+
+
+Lemma apply_InDep_app : forall l l0 l1 , InDep l -> l = l0++l1 -> 1 < size l1 -> InDep l1.
+Proof.
+intros.  apply : InDep_app;auto. rewrite H0 in H. eauto. 
+Qed.
+
+Lemma OutDep_app : forall l0 l1, OutDep (l0 ++ l1) -> 1 < size l1 -> OutDep l1.
+Proof.
+elim. rewrite /=. done.
+move => a l IH l1. rewrite cat_cons. move => H. inversion H. subst.
+case : l H2 H IH.  rewrite /=. move => <-. done. 
+move => a0 l. rewrite cat_cons. case. move => <-. case : l.  case : l1. done. done. done. 
+intros. subst. rewrite H1 in H3. auto. 
+Qed.
+
+Lemma outdep0 : forall l0 l1, outdep (l0 ++ l1) -> if l0 is x::l0' then path IO_OO x l0' else true.
+Proof.
+rewrite /outdep. case;first done. 
+move => a l l1. rewrite cat_cons. case : l;first done.  
+move => a0 l. rewrite cat_cons. rewrite -cat_cons. rewrite cat_path. by move/andP=>[]. 
+Qed.
+
+Lemma nil_ll : forall A (l0 l1 : seq A), nil = l0 ++ l1 -> l0 = nil /\ l1 = nil.
+Proof.
+move => A. elim.
+- case. done. done. 
+- rewrite /=. done. 
+Qed.
+
+Check list_ind.
+
+
+Lemma apply_OutDep_app : forall l l0 l1 , OutDep l -> l = l0++l1 -> 1 < size l1-> OutDep l1.
+Proof.
+intros.  apply : OutDep_app;auto. rewrite H0 in H. eauto. 
+Qed.
+
+Lemma delete_middle : forall a0 l0 a l1 a1 P, exists_depP (fun m => nth false m (size l0) = false) P a0 (l0 ++ a::l1) a1 ->
+                      exists_dep P a0 (l0++l1) a1.
+Proof.
+intros. move : H => [] m [] H0 [] H1 H2. exists ((take (size l0) m)++(drop (size l0).+1 m)).
+rewrite size_cat size_take size_drop H0 !size_cat /=. have : size l0 < size l0 + (size l1).+1 by lia.
+move => H3. rewrite H3. split. lia. split;auto. move : H1. rewrite !split_mask //=. rewrite H2 /= mask_cat //=. 
+by rewrite size_take H0 size_cat /= H3. 
+Qed.
+
+
+Lemma apply_linear : forall g s_tr a_p a0 s a1, Linear g -> Tr s_tr g -> s_tr = a_p++(a0::s++[::a1]) -> same_ch a0 a1 -> exists_dep InDep a0 s a1 /\ exists_dep OutDep a0 s a1.
+Proof.
+intros. rewrite H1 in H0. eauto. 
+Qed.
+
+Lemma get_neigbor : forall (P : action -> action -> bool) a p x_end m, path P a ((mask m p)++[::x_end]) -> exists x_in, x_in \in (a::p) /\ P x_in x_end. 
+Proof. 
+intros. 
+case : (split_list (mask m p)) H. move =>->. rewrite /= andbC /=. intros. exists a. by rewrite inE eqxx /=.
+move => [] l' [] a0 Heqa2.  move : (Heqa2) =>->. rewrite -catA. rewrite cat_path /=.
+move/andP=> [] _ /andP => [] [] _. rewrite andbC /=. move => HH.
+have : a0 \in a::p. rewrite inE.  apply/orP. right. apply (@mem_mask _ _  m). 
+rewrite Heqa2. by rewrite mem_cat inE eqxx orbC. 
+intros. exists a0. by rewrite x. 
+Qed.
+
+Lemma IO_II_in_action : forall a0 (l : label), IO_II a0 l -> in_action (ptcp_to a0) l.
+Proof.
+move => a0 a1. rewrite /IO_II. move/orP=>[]. rewrite /IO. move/eqP=>->. apply in_action_from.
+rewrite /II. move/eqP=>->. apply in_action_to.
+Qed.
+
+Lemma in_split : forall (A : eqType) l (x : A), x \in l -> exists l0 l1, l = l0 ++ x::l1.
+Proof.
+move => A. elim. done.
+move => a l IH x. rewrite inE. move/orP=>[]. move/eqP=>->. exists nil. exists l. done. move/IH=> [] l0 [] l1 ->. exists (a::l0),l1. done. 
+Qed. 
+
+(*Can be simplified more*)
+Lemma in_label : forall (l : label), ptcp_from l.1 \in l.
+Proof.
+case. intros. rewrite /=. destruct a. simpl. done.
+Qed.
+
+Hint Resolve in_label.
+
+Lemma stepG_aux : forall g G l g', stepG g G l g' -> Linear g -> 
+forall a0 aa a1, Tr (a0 :: aa ++ [:: a1]) g' -> same_ch a0 a1 -> exists_dep InDep a0 aa a1 /\ exists_dep OutDep a0 aa a1.
+Proof.
+move => g G l g'  Hstep  Lg a aa a1 HG Hch.
+move : (label_linear Hstep Lg) =>LG. case : (Tr_or (a:: aa ++ ([:: a1])) G); first auto using (LG nil).
+   move => Hnot.  
+   move : (deletion Hstep HG Hnot)=> [] s0 [] s1 [] Heq [] Hg0 HG0.
+   case : (cons23 Heq). 
+   move => [] Hs0 Hs1;subst; simpl in *. have : Tr (([::l.1]) ++ (a::aa) ++  ([::a1])) g. by  simpl. move => Hg0'.  apply : Lg. apply : Hg0'. done. 
+   case; first ( move => [] Hs0 Hs1; subst; apply : (LG nil); simpl; eauto using Tr_app). 
+   move => [] s0' [] s1' [] Hs0 [] Hs1 Heqaa. subst. simpl in *. 
+   move : (@apply_linear _ _ nil a (s0' ++ (l.1)::s1') a1 Lg Hg0).  (*get that original g contains in/out chains*)
+   rewrite /= -!catA cat_cons. move => Hinout. move : (Hinout Logic.eq_refl Hch)=> [] Hin Hout. 
+   rewrite  -cat_cons -[_::_]cat0s in HG0. (*make it ready to by used with LG*)
+   split.
+   ** move : Hin => [] m [] Hsize [] Hin _. (*InDep*)
+      case Heqb : (nth false m (size s0')); last (apply : delete_middle; exists m; split;eauto). 
+      move : Hin. rewrite split_mask //= Heqb /=.
+
+
+      move/InDep_iff.
+      have : (a :: (mask (take (size s0') m) s0' ++ l.1 :: mask (drop (size s0').+1 m) s1') ++ [:: a1]) =
+             (((a :: (mask (take (size s0') m) s0' ++ [::l.1])) ++ (mask (drop (size s0').+1 m) s1') ++ [:: a1])).
+      by rewrite /= -!catA. move =>->.
+
+      move/indep0. move/get_neigbor=> [] x_in []. intros.
+
+      exfalso. apply/negP. eapply reduce_condition with (a':=x_in). apply : Hstep.   apply : HG0. 
+      by rewrite mem_cat a0 orbC. apply IO_II_in_action. done. 
+
+  ** move : Hout => [] m [] Hsize [] Hout _. (*OutDep*) 
+     case Heqb : (nth false m (size s0')); last (apply : delete_middle; exists m; split;eauto).
+     move : Hout. rewrite split_mask //= Heqb /=.
+
+     move/OutDep_iff.
+      have : (a :: (mask (take (size s0') m) s0' ++ l.1 :: mask (drop (size s0').+1 m) s1') ++ [:: a1]) =
+             (((a :: (mask (take (size s0') m) s0' ++ [::l.1])) ++ (mask (drop (size s0').+1 m) s1') ++ [:: a1])).
+      by rewrite /= -!catA. move =>->.
+
+      move/outdep0. move/get_neigbor=> [] x_in []. intros. 
+      rewrite /IO_OO in b. case : (orP b). intros.  exfalso. apply : negP. eapply reduce_condition with (a':= x_in). apply : Hstep.
+      apply : HG0. by rewrite mem_cat a0 orbC. move : a2. rewrite /IO. move/eqP=>->. auto.  
+
+      rewrite /OO. move/andP=> [] /eqP _ HH0. 
+      move : (in_split a0)=> [] l1 [] l2 Heq0. have : x_in \in [::] ++ a :: s0' by rewrite mem_cat a0 orbC. move => xin. Check reduce_condition. move : (@reduce_condition _ _ _ _ Hstep _ _ _ HG0 xin )=> not_act. 
+  simpl in HG0. rewrite -cat_cons Heq0 -catA in HG0. 
+      
+        move : (LG _ _ _ _ HG0 HH0) => [] HInm HOutm. move : HInm => [] mm [] Hsizem  [] HInm _.
+        move : HInm. move/InDep_iff. 
+     case : (split_list (mask mm l2)). move=>->. rewrite /= /II. move/eqP=> HHeq.  exfalso. apply :negP. apply : not_act. 
+        rewrite HHeq. apply/in_action_to.  
+     move => [] l' [] a2 Heq2. rewrite Heq2 -!catA -cat_cons. move/indep1. rewrite /= andbC /=. move => HIO_II.  exfalso. apply : negP. 
+     eapply reduce_condition with (a':=a2). apply Hstep. rewrite catA in HG0.  apply : HG0.
+     rewrite mem_cat. apply/orP. right. rewrite inE. apply/orP. right. apply (@mem_mask  _ _ mm). rewrite Heq2.
+     by rewrite mem_cat inE  eqxx orbC. apply IO_II_in_action.  done.
+Qed.
+
+
+Lemma stepG_linear : forall g G l g', stepG g G l g' -> Linear g -> Linear g'.
+Proof.
+move => g G l g'. elim.  
+- eauto using linear_sgmsg.
+- eauto using linear_branch.  
+- intros. rewrite /Linear. case.
+ * eauto using stepG_aux. 
+ * intros. simpl in H3. inversion H3;subst. apply : H0;eauto using linear_sgmsg. 
+- intros. rewrite /Linear. case.
+ * eauto using stepG_aux.
+ * intros. simpl in H3. inversion H3;subst.
+   move : (app_Forall3 H0)=>[] HH HH1.
+   case Heq : (n < size gs).
+  **  apply : HH;eauto using linear_branch.  
+  ** rewrite nth_default in H6; last lia.  inversion H6. by move : H7=> /nil_ll  => [] []. 
+Qed.
